general heap and fancy updates

veric/fancy_updates.v
@@ -1,233 +1,103 @@
 From stdpp Require Export coPset.
-(*From iris.algebra Require Import gmap auth agree gset coPset.*)
+From iris_ora.algebra Require Import gmap agree.
 From iris.proofmode Require Import proofmode.
 From iris_ora.logic Require Export own.
-From iris_ora.logic Require Import wsat.
-(*From iris.base_logic Require Export later_credits.*)
+From VST.veric Require Import wsat.
+(*From iris.base_logic Require Export later_credits.*) (* TODO *)
 From iris.prelude Require Import options.
 Export wsatGS.
 Import ouPred.
-Import le_upd_if.
 
-(** The definition of fancy updates (and in turn the logic built on top of it) is parameterized
-    by whether it supports elimination of laters via later credits or not.
-    This choice is necessary as the fancy update *with* later credits does *not* support
-    the interaction laws with the plainly modality in [BiFUpdPlainly]. While these laws are
-    seldomly used, support for them is required for backwards compatibility.
+Local Definition ouPred_fupd_def `{!wsatGS Σ} (E1 E2 : coPset) (P : iProp Σ) : iProp Σ :=
+  wsat ∗ ownE E1 ==∗ ◇ (wsat ∗ ownE E2 ∗ P).
+Local Definition ouPred_fupd_aux : seal (@ouPred_fupd_def). Proof. by eexists. Qed.
+Definition ouPred_fupd := ouPred_fupd_aux.(unseal).
+Global Arguments ouPred_fupd {Σ _}.
+Local Lemma ouPred_fupd_unseal `{!wsatGS Σ} : @fupd _ ouPred_fupd = ouPred_fupd_def.
+Proof. rewrite -ouPred_fupd_aux.(seal_eq) //. Qed.
 
-    Thus, the [invGS_gen] typeclass ("gen" for "generalized") is parameterized by
-    a parameter of type [has_lc] that determines whether later credits are
-    available or not. [invGS] is provided as a convenient notation for the default [HasLc].
-    We don't use that notation in this file to avoid confusion.
- *)
-Inductive has_lc := HasLc | HasNoLc.
-
-Class invGpreS (Σ : gFunctors) : Set := InvGpreS {
-  invGpreS_wsat : wsatGpreS Σ;
-  invGpreS_lc : lcGpreS Σ;
-}.
-
-Class invGS_gen (hlc : has_lc) (Σ : gFunctors) : Set := InvG {
-  invGS_wsat : wsatGS Σ;
-  invGS_lc : lcGS Σ;
-}.
-Global Hint Mode invGS_gen - - : typeclass_instances.
-Global Hint Mode invGpreS - : typeclass_instances.
-Local Existing Instances invGpreS_wsat invGpreS_lc.
-(* [invGS_lc] needs to be global in order to enable the use of lemmas like [lc_split]
-   that require [lcGS], and not [invGS].
-   [invGS_wsat] also needs to be global as the lemmas in [invariants.v] require it. *)
-Global Existing Instances invGS_lc invGS_wsat.
-
-Notation invGS := (invGS_gen HasLc).
-
-Definition invΣ : gFunctors :=
-  #[wsatΣ; lcΣ].
-Global Instance subG_invΣ {Σ} : subG invΣ Σ → invGpreS Σ.
-Proof. solve_inG. Qed.
-
-Local Definition uPred_fupd_def `{!invGS_gen hlc Σ} (E1 E2 : coPset) (P : iProp Σ) : iProp Σ :=
-  wsat ∗ ownE E1 -∗ le_upd_if (if hlc is HasLc then true else false) (◇ (wsat ∗ ownE E2 ∗ P)).
-Local Definition uPred_fupd_aux : seal (@uPred_fupd_def). Proof. by eexists. Qed.
-Definition uPred_fupd := uPred_fupd_aux.(unseal).
-Global Arguments uPred_fupd {hlc Σ _}.
-Local Lemma uPred_fupd_unseal `{!invGS_gen hlc Σ} : @fupd _ uPred_fupd = uPred_fupd_def.
-Proof. rewrite -uPred_fupd_aux.(seal_eq) //. Qed.
-
-Lemma uPred_fupd_mixin `{!invGS_gen hlc Σ} : BiFUpdMixin (uPredI (iResUR Σ)) uPred_fupd.
+Lemma ouPred_fupd_mixin `{!wsatGS Σ} : BiFUpdMixin (ouPredI (iResUR Σ)) ouPred_fupd.
 Proof.
   split.
-  - rewrite uPred_fupd_unseal. solve_proper.
+  - rewrite ouPred_fupd_unseal. solve_proper.
   - intros E1 E2 (E1''&->&?)%subseteq_disjoint_union_L.
-    rewrite uPred_fupd_unseal /uPred_fupd_def ownE_op //.
+    rewrite ouPred_fupd_unseal /ouPred_fupd_def ownE_op //.
     by iIntros "($ & $ & HE) !> !> [$ $] !> !>" .
-  - rewrite uPred_fupd_unseal.
+  - rewrite ouPred_fupd_unseal.
     iIntros (E1 E2 P) ">H [Hw HE]". iApply "H"; by iFrame.
-  - rewrite uPred_fupd_unseal.
+  - rewrite ouPred_fupd_unseal.
     iIntros (E1 E2 P Q HPQ) "HP HwE". rewrite -HPQ. by iApply "HP".
-  - rewrite uPred_fupd_unseal. iIntros (E1 E2 E3 P) "HP HwE".
+  - rewrite ouPred_fupd_unseal. iIntros (E1 E2 E3 P) "HP HwE".
     iMod ("HP" with "HwE") as ">(Hw & HE & HP)". iApply "HP"; by iFrame.
-  - intros E1 E2 Ef P HE1Ef. rewrite uPred_fupd_unseal /uPred_fupd_def ownE_op //.
+  - intros E1 E2 Ef P HE1Ef. rewrite ouPred_fupd_unseal /ouPred_fupd_def ownE_op //.
     iIntros "Hvs (Hw & HE1 &HEf)".
     iMod ("Hvs" with "[Hw HE1]") as ">($ & HE2 & HP)"; first by iFrame.
     iDestruct (ownE_op' with "[HE2 HEf]") as "[? $]"; first by iFrame.
     iIntros "!> !>". by iApply "HP".
-  - rewrite uPred_fupd_unseal /uPred_fupd_def. by iIntros (????) "[HwP $]".
+  - rewrite ouPred_fupd_unseal /ouPred_fupd_def. by iIntros (????) "[HwP $]".
 Qed.
-Global Instance uPred_bi_fupd `{!invGS_gen hlc Σ} : BiFUpd (uPredI (iResUR Σ)) :=
-  {| bi_fupd_mixin := uPred_fupd_mixin |}.
+Global Instance ouPred_bi_fupd `{!wsatGS Σ} : BiFUpd (ouPredI (iResUR Σ)) :=
+  {| bi_fupd_mixin := ouPred_fupd_mixin |}.
 
-Global Instance uPred_bi_bupd_fupd `{!invGS_gen hlc Σ} : BiBUpdFUpd (uPredI (iResUR Σ)).
-Proof. rewrite /BiBUpdFUpd uPred_fupd_unseal. by iIntros (E P) ">? [$ $] !> !>". Qed.
+Global Instance ouPred_bi_bupd_fupd `{!wsatGS Σ} : BiBUpdFUpd (ouPredI (iResUR Σ)).
+Proof. rewrite /BiBUpdFUpd ouPred_fupd_unseal. by iIntros (E P) ">? [$ $] !> !>". Qed.
 
-(** The interaction laws with the plainly modality are only supported when
-  we opt out of the support for later credits. *)
-Global Instance uPred_bi_fupd_plainly_no_lc `{!invGS_gen HasNoLc Σ} :
-  BiFUpdPlainly (uPredI (iResUR Σ)).
+(*Global Instance ouPred_bi_fupd_plainly `{!wsatGS Σ} : BiFUpdPlainly (ouPredI (iResUR Σ)).
 Proof.
-  split; rewrite uPred_fupd_unseal /uPred_fupd_def.
-  - iIntros (E P) "H [Hw HE]".
+  split.
+  - rewrite ouPred_fupd_unseal /ouPred_fupd_def. iIntros (E P) "H [Hw HE]".
     iAssert (◇ ■ P)%I as "#>HP".
     { by iMod ("H" with "[$]") as "(_ & _ & HP)". }
     by iFrame.
-  - iIntros (E P Q) "[H HQ] [Hw HE]".
+  - rewrite ouPred_fupd_unseal /ouPred_fupd_def. iIntros (E P Q) "[H HQ] [Hw HE]".
     iAssert (◇ ■ P)%I as "#>HP".
     { by iMod ("H" with "HQ [$]") as "(_ & _ & HP)". }
     by iFrame.
-  - iIntros (E P) "H [Hw HE]".
+  - rewrite ouPred_fupd_unseal /ouPred_fupd_def. iIntros (E P) "H [Hw HE]".
     iAssert (▷ ◇ ■ P)%I as "#HP".
     { iNext. by iMod ("H" with "[$]") as "(_ & _ & HP)". }
     iFrame. iIntros "!> !> !>". by iMod "HP".
-  - iIntros (E A Φ) "HΦ [Hw HE]".
+  - rewrite ouPred_fupd_unseal /ouPred_fupd_def. iIntros (E A Φ) "HΦ [Hw HE]".
     iAssert (◇ ■ ∀ x : A, Φ x)%I as "#>HP".
     { iIntros (x). by iMod ("HΦ" with "[$Hw $HE]") as "(_&_&?)". }
     by iFrame.
-Qed.
+Qed.*)
 
-(** Note: the [_no_lc] soundness lemmas also allow generating later credits, but
-  these cannot be used for anything. They are merely provided to enable making
-  the adequacy proof generic in whether later credits are used. *)
-Lemma fupd_plain_soundness_no_lc `{!invGpreS Σ} E1 E2 (P: iProp Σ) `{!Plain P} m :
-  (∀ `{Hinv: !invGS_gen HasNoLc Σ}, £ m ⊢ |={E1,E2}=> P) → ⊢ P.
+(* What's the linear equivalent of this?
+Lemma fupd_plain_soundness `{!invGpreS Σ} E1 E2 (P: iProp Σ) `{!Plain P} :
+  (∀ `{Hinv: !wsatGS Σ}, ⊢ |={E1,E2}=> P) → ⊢ P.
 Proof.
-  iIntros (Hfupd). apply later_soundness. iMod wsat_alloc as (Hw) "[Hw HE]".
-  (* We don't actually want any credits, but we need the [lcGS]. *)
-  iMod (later_credits.le_upd.lc_alloc m) as (Hc) "[_ Hc]".
-  set (Hi := InvG HasNoLc _ Hw Hc).
-  iAssert (|={⊤,E2}=> P)%I with "[Hc]" as "H" .
-  { iMod (fupd_mask_subseteq E1) as "_"; first done. iApply Hfupd; last done. }
-  rewrite uPred_fupd_unseal /uPred_fupd_def.
-  iMod ("H" with "[$]") as "[Hw [HE >H']]"; iFrame.
+  iIntros (Hfupd). apply later_soundness. apply bupd_plain_soundness; first by apply later_plain.
+  iMod wsat_alloc as (Hinv) "[Hw HE]".
+  iPoseProof Hfupd as "H".
+  rewrite (union_difference_L E1 ⊤); last done.
+  rewrite ownE_op; last by set_solver.
+  iDestruct "HE" as "[HE1 HE]".
+  rewrite ouPred_fupd_unseal /ouPred_fupd_def.
+  iMod ("H" with "[$]") as "[Hw [HE2 >H']]"; iFrame.
 Qed.
 
-Lemma step_fupdN_soundness_no_lc `{!invGpreS Σ} φ n m :
-  (∀ `{Hinv: !invGS_gen HasNoLc Σ}, £ m ⊢@{iPropI Σ} |={⊤,∅}=> |={∅}▷=>^n ⌜ φ ⌝) →
+Lemma step_fupdN_soundness `{!invGpreS Σ} φ n :
+  (∀ `{Hinv: !wsatGS Σ}, ⊢@{iPropI Σ} |={⊤,∅}=> |={∅}▷=>^n ⌜ φ ⌝) →
   φ.
 Proof.
   intros Hiter.
   apply (soundness (M:=iResUR Σ) _  (S n)); simpl.
-  apply (fupd_plain_soundness_no_lc ⊤ ⊤ _ m)=> Hinv. iIntros "Hc".
+  apply (fupd_plain_soundness ⊤ ⊤ _)=> Hinv.
   iPoseProof (Hiter Hinv) as "H". clear Hiter.
-  iApply fupd_plainly_mask_empty. iSpecialize ("H" with "Hc").
-  iMod (step_fupdN_plain with "H") as "H". iMod "H". iModIntro.
+  iApply fupd_plainly_mask_empty. iMod "H".
+  iMod (step_fupdN_plain with "H") as "H". iModIntro.
   rewrite -later_plainly -laterN_plainly -later_laterN laterN_later.
   iNext. iMod "H" as %Hφ. auto.
 Qed.
 
-Lemma step_fupdN_soundness_no_lc' `{!invGpreS Σ} φ n m :
-  (∀ `{Hinv: !invGS_gen HasNoLc Σ}, £ m ⊢@{iPropI Σ} |={⊤}[∅]▷=>^n ⌜ φ ⌝) →
+Lemma step_fupdN_soundness' `{!invGpreS Σ} φ n :
+  (∀ `{Hinv: !wsatGS Σ}, ⊢@{iPropI Σ} |={⊤}[∅]▷=>^n ⌜ φ ⌝) →
   φ.
 Proof.
-  iIntros (Hiter). eapply (step_fupdN_soundness_no_lc _ n m)=>Hinv.
-  iIntros "Hcred". destruct n as [|n].
+  iIntros (Hiter). eapply (step_fupdN_soundness _ n)=>Hinv. destruct n as [|n].
   { by iApply fupd_mask_intro_discard; [|iApply (Hiter Hinv)]. }
-   simpl in Hiter |- *. iMod (Hiter with "Hcred") as "H". iIntros "!>!>!>".
+   simpl in Hiter |- *. iMod Hiter as "H". iIntros "!>!>!>".
   iMod "H". clear. iInduction n as [|n] "IH"; [by iApply fupd_mask_intro_discard|].
   simpl. iMod "H". iIntros "!>!>!>". iMod "H". by iApply "IH".
-Qed.
-
-(** Later credits: the laws are only available when we opt into later credit support.*)
-
-(** [lc_fupd_elim_later] allows to eliminate a later from a hypothesis at an update.
-  This is typically used as [iMod (lc_fupd_elim_later with "Hcredit HP") as "HP".],
-  where ["Hcredit"] is a credit available in the context and ["HP"] is the
-  assumption from which a later should be stripped. *)
-Lemma lc_fupd_elim_later `{!invGS_gen HasLc Σ} E P :
-   £ 1 -∗ (▷ P) -∗ |={E}=> P.
-Proof.
-  iIntros "Hf Hupd".
-  rewrite uPred_fupd_unseal /uPred_fupd_def.
-  iIntros "[$ $]". iApply (le_upd_later with "Hf").
-  iNext. by iModIntro.
-Qed.
-
-(** If the goal is a fancy update, this lemma can be used to make a later appear
-  in front of it in exchange for a later credit.
-  This is typically used as [iApply (lc_fupd_add_later with "Hcredit")],
-  where ["Hcredit"] is a credit available in the context. *)
-Lemma lc_fupd_add_later `{!invGS_gen HasLc Σ} E1 E2 P :
-  £ 1 -∗ (▷ |={E1, E2}=> P) -∗ |={E1, E2}=> P.
-Proof.
-  iIntros "Hf Hupd". iApply (fupd_trans E1 E1).
-  iApply (lc_fupd_elim_later with "Hf Hupd").
-Qed.
-
-Lemma fupd_soundness_lc `{!invGpreS Σ} n E1 E2 φ :
-  (∀ `{Hinv: !invGS_gen HasLc Σ}, £ n ⊢@{iPropI Σ} |={E1,E2}=> ⌜φ⌝) → φ.
-Proof.
-  iIntros (Hfupd). eapply (lc_soundness (S n)). intros Hc.
-  rewrite lc_succ.
-  iIntros "[Hone Hn]". rewrite -le_upd_trans. iApply bupd_le_upd.
-  iMod wsat_alloc as (Hw) "[Hw HE]".
-  set (Hi := InvG HasLc _ Hw Hc).
-  iAssert (|={⊤,E2}=> ⌜φ⌝)%I with "[Hn]" as "H".
-  { iMod (fupd_mask_subseteq E1) as "_"; first done. by iApply (Hfupd Hi). }
-  rewrite uPred_fupd_unseal /uPred_fupd_def.
-  iModIntro. iMod ("H" with "[$Hw $HE]") as "H".
-  iPoseProof (except_0_into_later with "H") as "H".
-  iApply (le_upd_later with "Hone"). iNext.
-  iDestruct "H" as "(_ & _ & $)".
-Qed.
-
-Lemma step_fupdN_soundness_lc `{!invGpreS Σ} φ n m :
-  (∀ `{Hinv: !invGS_gen HasLc Σ}, £ m ⊢@{iPropI Σ} |={⊤,∅}=> |={∅}▷=>^n ⌜ φ ⌝) →
-  φ.
-Proof.
-  intros Hiter. eapply (fupd_soundness_lc (m + n)); [apply _..|].
-  iIntros (Hinv) "Hlc". rewrite lc_split.
-  iDestruct "Hlc" as "[Hm Hn]". iMod (Hiter with "Hm") as "Hupd".
-  clear Hiter.
-  iInduction n as [|n] "IH"; simpl.
-  - by iModIntro.
-  - rewrite lc_succ. iDestruct "Hn" as "[Hone Hn]".
-    iMod "Hupd". iMod (lc_fupd_elim_later with "Hone Hupd") as "> Hupd".
-    by iApply ("IH" with "Hn Hupd").
-Qed.
-
-Lemma step_fupdN_soundness_lc' `{!invGpreS Σ} φ n m :
-  (∀ `{Hinv: !invGS_gen hlc Σ}, £ m ⊢@{iPropI Σ} |={⊤}[∅]▷=>^n ⌜ φ ⌝) →
-  φ.
-Proof.
-  intros Hiter. eapply (fupd_soundness_lc (m + n) ⊤ ⊤); [apply _..|].
-  iIntros (Hinv) "Hlc". rewrite lc_split.
-  iDestruct "Hlc" as "[Hm Hn]". iPoseProof (Hiter with "Hm") as "Hupd".
-  clear Hiter.
-  iInduction n as [|n] "IH"; simpl.
-  - by iModIntro.
-  - rewrite lc_succ. iDestruct "Hn" as "[Hone Hn]".
-    iMod "Hupd". iMod (lc_fupd_elim_later with "Hone Hupd") as "> Hupd".
-    by iApply ("IH" with "Hn Hupd").
-Qed.
-
-(** Generic soundness lemma for the fancy update, parameterized by [use_credits]
-  on whether to use credits or not. *)
-Lemma step_fupdN_soundness_gen `{!invGpreS Σ} (φ : Prop) (hlc : has_lc) (n m : nat) :
-  (∀ `{Hinv : invGS_gen hlc Σ},
-    £ m ={⊤,∅}=∗ |={∅}▷=>^n ⌜φ⌝) →
-  φ.
-Proof.
-  destruct hlc.
-  - apply step_fupdN_soundness_lc.
-  - apply step_fupdN_soundness_no_lc.
-Qed.
-
+Qed.*)
