veric/algebras.v
@@ -1,0 +1,181 @@
+(* General extra lemmas about algebras of interest, extracted from iris.base_logic.algebra *)
+From iris_ora.logic Require Import logic.
+From VST.veric Require Import dfrac view gmap_view.
+
+Section oupred.
+  Context {M : uora}.
+
+  (* Force implicit argument M *)
+  Notation "P ⊢ Q" := (bi_entails (PROP:=ouPredI M) P Q).
+  Notation "P ⊣⊢ Q" := (equiv (A:=ouPredI M) P%I Q%I).
+  Notation "⊢ Q" := (bi_entails (PROP:=ouPredI M) True Q).
+
+Section view.
+  Context {A} {B : uora} (rel : view_rel A B).
+  Implicit Types a : A.
+  Implicit Types ag : option (share * agree A).
+  Implicit Types b : B.
+  Implicit Types x y : view rel.
+
+  Context (view_rel_order : ∀n a b1 b2, b1 ≼ₒ{n} b2 → rel n a b2 → rel n a b1).
+
+  Local Canonical Structure viewR := (view.viewR rel view_rel_order).
+
+  Lemma view_both_dfrac_validI_1 (relI : ouPred M) dq a b :
+    (∀ n (x : M), rel n a b → relI n x) →
+    ✓ (●V{dq} a ⋅ ◯V b : viewR) ⊢ ⌜✓dq⌝ ∧ relI.
+  Proof.
+    intros Hrel. ouPred.unseal. split=> n x _ /=.
+    rewrite /ouPred_holds /= view_both_dfrac_validN. by move=> [? /Hrel].
+  Qed.
+  Lemma view_both_dfrac_validI_2 (relI : ouPred M) dq a b :
+    (∀ n (x : M), relI n x → rel n a b) →
+    ⌜✓dq⌝ ∧ relI ⊢ ✓ (●V{dq} a ⋅ ◯V b : viewR).
+  Proof.
+    intros Hrel. ouPred.unseal. split=> n x _ /=.
+    rewrite /ouPred_holds /= view_both_dfrac_validN. by move=> [? /Hrel].
+  Qed.
+  Lemma view_both_dfrac_validI (relI : ouPred M) dq a b :
+    (∀ n (x : M), rel n a b ↔ relI n x) →
+    ✓ (●V{dq} a ⋅ ◯V b : viewR) ⊣⊢ ⌜✓dq⌝ ∧ relI.
+  Proof.
+    intros. apply (anti_symm _);
+      [apply view_both_dfrac_validI_1|apply view_both_dfrac_validI_2]; naive_solver.
+  Qed.
+
+  Lemma view_both_validI_1 (relI : ouPred M) a b :
+    (∀ n (x : M), rel n a b → relI n x) →
+    ✓ (●V a ⋅ ◯V b : viewR) ⊢ relI.
+  Proof. intros. by rewrite view_both_dfrac_validI_1 // bi.and_elim_r. Qed.
+  Lemma view_both_validI_2 (relI : ouPred M) a b :
+    (∀ n (x : M), relI n x → rel n a b) →
+    relI ⊢ ✓ (●V a ⋅ ◯V b : viewR).
+  Proof.
+    intros. rewrite -view_both_dfrac_validI_2 //.
+    apply bi.and_intro; [|done]. by apply bi.pure_intro.
+  Qed.
+  Lemma view_both_validI (relI : ouPred M) a b :
+    (∀ n (x : M), rel n a b ↔ relI n x) →
+    ✓ (●V a ⋅ ◯V b : viewR) ⊣⊢ relI.
+  Proof.
+    intros. apply (anti_symm _);
+      [apply view_both_validI_1|apply view_both_validI_2]; naive_solver.
+  Qed.
+
+  Lemma view_auth_dfrac_validI (relI : ouPred M) dq a :
+    (∀ n (x : M), relI n x ↔ rel n a ε) →
+    ✓ (●V{dq} a : viewR) ⊣⊢ ⌜✓dq⌝ ∧ relI.
+  Proof.
+    intros. rewrite -(right_id ε op (●V{dq} a)). by apply view_both_dfrac_validI.
+  Qed.
+  Lemma view_auth_validI (relI : ouPred M) a :
+    (∀ n (x : M), relI n x ↔ rel n a ε) →
+    ✓ (●V a : viewR) ⊣⊢ relI.
+  Proof. intros. rewrite -(right_id ε op (●V a)). by apply view_both_validI. Qed.
+
+  Lemma view_frag_validI (relI : ouPred M) b :
+    (∀ n (x : M), relI n x ↔ ∃ a, rel n a b) →
+    ✓ (◯V b : viewR) ⊣⊢ relI.
+  Proof. ouPred.unseal=> Hrel. split=> n x _. by rewrite Hrel. Qed.
+End view.
+
+(*From iris.algebra Require Import auth excl_auth.
+
+Section auth.
+  Context {A : uora}.
+  Implicit Types a b : A.
+  Implicit Types x y : auth A.
+
+  Lemma auth_auth_dfrac_validI dq a : ✓ (●{dq} a) ⊣⊢ ⌜✓dq⌝ ∧ ✓ a.
+  Proof.
+    apply view_auth_dfrac_validI=> n. ouPred.unseal; split; [|by intros [??]].
+    split; [|done]. apply uora_unit_leastN.
+  Qed.
+  Lemma auth_auth_validI a : ✓ (● a) ⊣⊢ ✓ a.
+  Proof.
+    by rewrite auth_auth_dfrac_validI bi.pure_True // left_id.
+  Qed.
+
+  Lemma auth_frag_validI a : ✓ (◯ a) ⊣⊢ ✓ a.
+  Proof.
+    apply view_frag_validI=> n x.
+    rewrite auth_view_rel_exists. by ouPred.unseal.
+  Qed.
+
+  Lemma auth_both_dfrac_validI dq a b :
+    ✓ (●{dq} a ⋅ ◯ b) ⊣⊢ ⌜✓dq⌝ ∧ (∃ c, a ≡ b ⋅ c) ∧ ✓ a.
+  Proof. apply view_both_dfrac_validI=> n. by ouPred.unseal. Qed.
+  Lemma auth_both_validI a b :
+    ✓ (● a ⋅ ◯ b) ⊣⊢ (∃ c, a ≡ b ⋅ c) ∧ ✓ a.
+  Proof.
+    by rewrite auth_both_dfrac_validI bi.pure_True // left_id.
+  Qed.
+
+End auth.
+
+Section excl_auth.
+  Context {A : ofe}.
+  Implicit Types a b : A.
+
+  Lemma excl_auth_agreeI a b : ✓ (●E a ⋅ ◯E b) ⊢ (a ≡ b).
+  Proof.
+    rewrite auth_both_validI bi.and_elim_l.
+    apply bi.exist_elim=> -[[c|]|];
+      by rewrite option_equivI /= excl_equivI //= bi.False_elim.
+  Qed.
+End excl_auth.
+
+Section dfrac_agree.
+  Context {A : ofe}.
+  Implicit Types a b : A.
+
+  Lemma dfrac_agree_validI dq a : ✓ (to_dfrac_agree dq a) ⊣⊢ ⌜✓ dq⌝.
+  Proof.
+    rewrite prod_validI /= ouPred.discrete_valid. apply bi.entails_anti_sym.
+    - by rewrite bi.and_elim_l.
+    - apply bi.and_intro; first done. etrans; last apply to_agree_validI.
+      apply bi.True_intro.
+  Qed.
+
+  Lemma dfrac_agree_validI_2 dq1 dq2 a b :
+    ✓ (to_dfrac_agree dq1 a ⋅ to_dfrac_agree dq2 b) ⊣⊢ ⌜✓ (dq1 ⋅ dq2)⌝ ∧ (a ≡ b).
+  Proof.
+    rewrite prod_validI /= ouPred.discrete_valid to_agree_op_validI //.
+  Qed.
+
+  Lemma frac_agree_validI q a : ✓ (to_frac_agree q a) ⊣⊢ ⌜(q ≤ 1)%Qp⌝.
+  Proof.
+    rewrite dfrac_agree_validI dfrac_valid_own //.
+  Qed.
+
+  Lemma frac_agree_validI_2 q1 q2 a b :
+    ✓ (to_frac_agree q1 a ⋅ to_frac_agree q2 b) ⊣⊢ ⌜(q1 + q2 ≤ 1)%Qp⌝ ∧ (a ≡ b).
+  Proof.
+    rewrite dfrac_agree_validI_2 dfrac_valid_own //.
+  Qed.
+End dfrac_agree.*)
+
+Section gmap_view.
+  Context {K : Type} `{Countable K} {V : ofe}.
+  Implicit Types (m : gmap K V) (k : K) (dq : dfrac) (v : V).
+
+  Lemma gmap_view_both_validI m k dq v :
+    ✓ (gmap_view_auth (DfracOwn Tsh) m ⋅ gmap_view_frag k dq v) ⊢
+    ✓ dq ∧ m !! k ≡ Some v.
+  Proof.
+    rewrite /gmap_view_auth /gmap_view_frag. apply view_both_validI_1.
+    intros n a. ouPred.unseal. apply gmap_view.gmap_view_rel_lookup.
+  Qed.
+
+  Lemma gmap_view_frag_op_validI k dq1 dq2 v1 v2 :
+    ✓ (gmap_view_frag k dq1 v1 ⋅ gmap_view_frag k dq2 v2) ⊣⊢
+    ✓ (dq1 ⋅ dq2) ∧ v1 ≡ v2.
+  Proof.
+    rewrite /gmap_view_frag -view_frag_op. apply view_frag_validI=> n x.
+    rewrite gmap_view.gmap_view_rel_exists singleton_op singleton_validN.
+    rewrite pair_validN to_agree_op_validN. by ouPred.unseal.
+  Qed.
+
+End gmap_view.
+
+End oupred.
